semantics/semantics.v
@@ -590,12 +590,10 @@ Definition updateNV_arr (N: nvmem) (i: el_loc) (a: array) (v: value) :=
 Definition updatemaps (N: nvmem) (N': nvmem): nvmem :=
   match N, N' with
     NonVol m D, NonVol m' D' => NonVol
-  (fun j =>
-     match m j with
-     error => m' j
-     | x => x
-     end
-  )
+   (fun j =>
+      if (j \in D)
+          then (m j)
+          else (m' j))
   (D ++ D') (*inclusion of duplicates*)
   end.
 Notation "m1 'U!' m2" := (updatemaps m1 m2) (at level 100).
@@ -774,12 +772,21 @@ Definition single_com_i (C: iconf) :=
 WAR variables
  *)
 
-Fixpoint readobs_loc (R: readobs): (seq loc) := 
+(*Fixpoint readobs_wvs (R: readobs): (seq loc) := 
   match R with
     nil => nil
-| (r::rs) => match r with
-             (location, _) => location :: (readobs_loc rs)
-           end
+  | (r::rs) => (fst r) :: (readobs_wvs rs)
+  end.*)
+
+Definition getwvs (l: loc) :=
+  match l with
+    inl x => [::l]
+  | inr (El a _) => (generate_locs a) end.
+
+Fixpoint readobs_wvs (R: readobs): (seq loc) := 
+  match R with
+    nil => nil
+  | (r::rs) => getwvs(fst r) ++ (readobs_wvs rs)
   end.
 
 
@@ -910,7 +917,7 @@ CheckPoint: forall(N: nvmem)
     cceval_w (N, V, Ins (asgn_sv x e))
              (Obs r :: nil)
              ((updateNV_sv N x v), V, Ins skip)
-             ([:: inl x],  (readobs_loc r), (remove (readobs_loc r) [:: inl x]))
+             ([:: inl x],  (readobs_wvs r), (remove (readobs_wvs r) [:: inl x]))
 | V_Assign: forall(x: smallvar) (N: nvmem) (mapV: mem) (e: exp) (r: readobs) (v: value),
     eeval N (Vol mapV) e r v ->
     isV(x) -> (*checks x is correct type for V memory*)
@@ -918,7 +925,7 @@ CheckPoint: forall(N: nvmem)
     cceval_w (N, (Vol mapV), Ins (asgn_sv x e)) 
              (Obs r :: nil)
              (N, (Vol ((inl x) |-> v ; mapV)), Ins skip)
-             (nil,  (readobs_loc r), nil)
+             (nil,  (readobs_wvs r), nil)
 | Assign_Arr: forall (N: nvmem) (V: vmem)
                (a: array)
                (ei: exp)
@@ -937,7 +944,7 @@ CheckPoint: forall(N: nvmem)
     cceval_w (N, V, Ins (asgn_arr a ei e))
            ((Obs (app ri r)) :: nil)
            ((updateNV_arr N element a v), V, Ins skip)
-           ([:: inr element], (readobs_loc (cat ri r)), (remove (readobs_loc (cat ri r)) [:: inr element]))
+           ([:: inr element], (readobs_wvs (cat ri r)), (remove (readobs_wvs (cat ri r)) [:: inr element]))
 (*valuability and inboundedness of vindex are checked in sameindex*)
 | Skip: forall(N: nvmem)
          (V: vmem)
@@ -962,14 +969,14 @@ CheckPoint: forall(N: nvmem)
          (r: readobs)
          (c1 c2: command),
     eeval N V e r true -> (*yuh doy not writing anything in eeval*)
-    cceval_w (N, V, (TEST e THEN c1 ELSE c2)) ((Obs r)::nil) (N, V, c1) (nil, (readobs_loc r), nil)
+    cceval_w (N, V, (TEST e THEN c1 ELSE c2)) ((Obs r)::nil) (N, V, c1) (nil, (readobs_wvs r), nil)
 | If_F: forall(N: nvmem)
          (V: vmem)
          (e: exp)
          (r: readobs)
          (c1 c2: command),
     eeval N V e r false ->
-    cceval_w (N, V, (TEST e THEN c1 ELSE c2)) ((Obs r)::nil) (N, V, c2) (nil, (readobs_loc r), nil).
+    cceval_w (N, V, (TEST e THEN c1 ELSE c2)) ((Obs r)::nil) (N, V, c2) (nil, (readobs_wvs r), nil).
 
 Definition append_write (W1 W2: the_write_stuff) :=
   ((getwt W1) ++ (getwt W2), (getrd W1) ++ (getrd W2), (getfstwt W1) ++ (remove (getrd W1) (getfstwt W2))).
@@ -1000,7 +1007,7 @@ Inductive iceval_w: iconf -> obseq -> iconf -> the_write_stuff -> Prop :=
     iceval_w (k, N, V, Ins (asgn_sv x e))
            [:: Obs r]
            (k, (updateNV_sv N x v), V, Ins skip)
-           ([:: inl x],  (readobs_loc r), (remove (readobs_loc r) [:: inl x]))
+           ([:: inl x],  (readobs_wvs r), (remove (readobs_wvs r) [:: inl x]))
 | CP_V_Assign: forall(k: context) (x: smallvar) (N: nvmem) (mapV: mem) (e: exp) (r: readobs) (v: value),
     eeval N (Vol mapV) e r v ->
     isV(x) -> (*checks x is correct type for V memory*)
@@ -1008,7 +1015,7 @@ Inductive iceval_w: iconf -> obseq -> iconf -> the_write_stuff -> Prop :=
     iceval_w (k, N, (Vol mapV), Ins (asgn_sv x e))
            [:: Obs r]
            (k, N, (Vol ((inl x) |-> v ; mapV)), Ins skip)
-             (nil,  (readobs_loc r), nil)
+             (nil,  (readobs_wvs r), nil)
 | CP_Assign_Arr: forall (k: context) (N: nvmem) (V: vmem)
                (a: array)
                (ei: exp)
@@ -1025,7 +1032,7 @@ Inductive iceval_w: iconf -> obseq -> iconf -> the_write_stuff -> Prop :=
     iceval_w (k, N, V, Ins (asgn_arr a ei e))
            [:: Obs (ri++r)]
            (k, (updateNV_arr N element a v), V, Ins skip)
-           ([:: inr element], (readobs_loc (cat ri r)), (remove  (readobs_loc (cat ri r)) [:: inr element]))
+           ([:: inr element], (readobs_wvs (cat ri r)), (remove  (readobs_wvs (cat ri r)) [:: inr element]))
 | CP_Skip: forall(k: context) (N: nvmem)
          (V: vmem)
          (c: command),
@@ -1044,13 +1051,13 @@ Inductive iceval_w: iconf -> obseq -> iconf -> the_write_stuff -> Prop :=
          (r: readobs)
          (c1 c2: command),
     eeval N V e r true -> 
-    iceval_w (k, N, V, (TEST e THEN c1 ELSE c2)) ((Obs r)::nil) (k, N, V, c1) (nil, (readobs_loc r), nil)
+    iceval_w (k, N, V, (TEST e THEN c1 ELSE c2)) ((Obs r)::nil) (k, N, V, c1) (nil, (readobs_wvs r), nil)
 |CP_If_F: forall(k: context) (N: nvmem) (V: vmem)
          (e: exp)
          (r: readobs)
          (c1 c2: command),
     eeval N V e r false ->
-    iceval_w (k, N, V, (TEST e THEN c1 ELSE c2)) ((Obs r)::nil) (k, N, V, c2) (nil, (readobs_loc r), nil).
+    iceval_w (k, N, V, (TEST e THEN c1 ELSE c2)) ((Obs r)::nil) (k, N, V, c2) (nil, (readobs_wvs r), nil).
 (*CP_Reboot: I took out the equals premise and instead built it
 into the types because I didn't wanit to define a context equality function*)
 
